Move closLang pure up, and improve it slightly
It was defined in clos_remove, but is now moved to closLang for reuse in
other phases. It was unnecessarily restrictive of Letrecs, now fixed.

compiler/backend/clos_removeScript.sml
@@ -10,47 +10,6 @@ open indexedListsTheory
 
 val _ = new_theory"clos_remove";
 
-val pure_op_def = Define `
-  pure_op op ⇔
-    case op of
-      FFI _ => F
-    | SetGlobal _ => F
-    | AllocGlobal => F
-    | RefByte => F
-    | RefArray => F
-    | UpdateByte => F
-    | Ref => F
-    | Update => F
-    | _ => T
-`;
-
-(* pure e means e can neither raise an exception nor side-effect the state *)
-val pure_def = tDefine "pure" `
-  (pure (Var _) ⇔ T)
-    ∧
-  (pure (If e1 e2 e3) ⇔ pure e1 ∧ pure e2 ∧ pure e3)
-    ∧
-  (pure (Let es e2) ⇔ EVERY pure es ∧ pure e2)
-    ∧
-  (pure (Raise _) ⇔ F)
-    ∧
-  (pure (Handle e1 _) ⇔ pure e1)
-    ∧
-  (pure (Tick _) ⇔ F)
-    ∧
-  (pure (Call _ _) ⇔ F)
-    ∧
-  (pure (App _ _ _) ⇔ F)
-    ∧
-  (pure (Fn _ _ _ _) ⇔ T)
-    ∧
-  (pure (Letrec _ _ fns x) ⇔ EVERY (λ(n,e). pure e) fns ∧ pure x)
-    ∧
-  (pure (Op opn es) ⇔ EVERY pure es ∧ pure_op opn)
-` (WF_REL_TAC `measure exp_size` >> simp[] >> rpt conj_tac >> rpt gen_tac >>
-   (Induct_on `es` ORELSE Induct_on `fns`) >> dsimp[exp_size_def] >>
-   rpt strip_tac >> res_tac >> simp[])
-
 val no_overlap_def = Define `
   (no_overlap 0 l <=> T) /\
   (no_overlap (SUC n) l <=>
